project: init part 1

Compiler9000.lean
@@ -1,1 +1,26 @@
-#eval "Hello, world!"
+import Lean
+
+inductive LambdaTerm where
+| num (val : Nat)
+| app (fn: LambdaTerm) (arg: LambdaTerm)
+| lambda (body: LambdaTerm)
+
+-- Q1.2
+def allFreeVariablesBoundBy : Nat -> LambdaTerm -> Bool
+| (n: Nat), LambdaTerm.num (val := m) => m <= n
+| (n: Nat), LambdaTerm.app (fn := fn) (arg := arg) => allFreeVariablesBoundBy n fn && allFreeVariablesBoundBy n arg
+| (n: Nat), LambdaTerm.lambda (body := t) => allFreeVariablesBoundBy n t
+
+def isClosedTerm (t: LambdaTerm): Prop := sorry
+theorem isClosedTermOfFreeVariablesBoundness (n: Nat) (t: LambdaTerm) (h: allFreeVariablesBoundBy n t): isClosedTerm t := sorry
+
+-- Q1.3
+def substitute (t: LambdaTerm) (index: Nat) (expr: LambdaTerm): LambdaTerm := sorry
+theorem closedTermSubstitutedEqClosedTerm (t: LambdaTerm) (h: isClosedTerm t) (index: Nat) (expr: LambdaTerm): substitute t index expr = t := sorry
+
+-- Q1.4
+def batchSubstitute (t: LambdaTerm) (startIndex: Nat) (exprs: List LambdaTerm): LambdaTerm := sorry
+-- theorem isClosedTerm.batchSubstitution (t: )
+-- case 0: t[] = t
+-- case 1: allFreeVariablesBoundBy i t → batchSubstitute t i [u] = t
+-- case 2: forall k ≥ 1, allFreeVariablesBoundBy i u_k, batchSubstitute t i [ u_0 … u_n] = substitute i u_0 (batchSubstitute t (i + 1) [ u_1 … u_n ])
